found a workaround to a strange bug

LeanLambdaLibMathlib/LambdaLib/testcases.lean
@@ -53,7 +53,8 @@ noncomputable def means'
 noncomputable def means (lvl : Nat) (ty : QTerm) : Option (QTerm → Prop) :=
   match lvl with
   | .zero => none -- some (fun _ ↦ False)
-  | .succ lvl' => means' (means lvl') ty
+  -- | .succ lvl' => means' (means lvl') ty
+  | .succ lvl' => runProg (means_prog (means lvl')) ty
 
 inductive means_ctx : QTerm → QTerm → Prop where
 | in_nil : means_ctx S.nil S.nil
@@ -63,6 +64,39 @@ inductive means_ctx : QTerm → QTerm → Prop where
   → s val
   → means_ctx <{S.pair} {env} {val}> <{S.cons} {ctx} {const (.natConst lvl)} {T}>
 
+macro "simp1" : tactic => `(tactic|
+  simp only [means, means', means_prog, runProg,
+    runProgDefinitionRet, runProgDefinitionRec, collectOptionDef]
+)
+macro "simp2" : tactic => `(tactic|
+  simp (disch := intros; lambda_solve; try trivial) only [PmatchDef1, PmatchDef2,
+    Pmatch2Def1, Pmatch2Def2, PifDef1, PifDef2]
+)
+
+example (SA A)
+  (rec1 : means 1 A = some SA)
+  : means 1 A = SA
+  := by
+  --
+  simp1
+  simp only [means, means', means_prog, runProg,
+    runProgDefinitionRet, runProgDefinitionRec, collectOptionDef] at rec1
+  rewrite [rec1]
+  --
+  sorry
+
+def mybind1 : Option α → (α → Option β) → Option β
+  | none,   _ => none
+  | some a, f => f a
+
+theorem gothere : @Option.bind = @mybind1 := by
+  ext X Y a b
+  cases a <;> trivial
+
+theorem goback : @mybind1 = @Option.bind := by
+  rw [gothere]
+
+-- set_option diagnostics true
 -- TODO: get this sort of things to work!
 example (SA SB A B)
   (rec1 : means 1 A = some SA)
@@ -70,12 +104,178 @@ example (SA SB A B)
   : means 1 <Pi {A} (λ a. {B})> = some (fun f ↦ ∀ a, SA a → SB <{f} {a}>)
   := by
   --
-  repeat (first
-    | simp only [means, means', means_prog]
-    | simp only [runProg, runProgDefinitionRet, runProgDefinitionRec, collectOptionDef]
-    | simp (disch := intros; lambda_solve; try trivial) only [PmatchDef1, PmatchDef2]
-    | simp (disch := intros; lambda_solve; try trivial) only [Pmatch2Def1, Pmatch2Def2]
-    | simp (disch := intros; lambda_solve; try trivial) only [PifDef1, PifDef2]
-  )
+  -- repeat (first
+  --   | simp only [means, means', means_prog]
+  --   | simp only [runProg, runProgDefinitionRet, runProgDefinitionRec, collectOptionDef]
+  --   | simp (disch := intros; lambda_solve; try trivial) only [PmatchDef1, PmatchDef2]
+  --   | simp (disch := intros; lambda_solve; try trivial) only [Pmatch2Def1, Pmatch2Def2]
+  --   | simp (disch := intros; lambda_solve; try trivial) only [PifDef1, PifDef2]
+  -- )
+  simp1
+  --
+  -- simp2
+  simp (maxDischargeDepth := 1) (disch := intros; lambda_solve; try trivial)
+    only [PmatchDef1, PmatchDef2, Pmatch2Def1, Pmatch2Def2, PifDef1, PifDef2]
+  simp1
+  -- OK, so if i get rid of the Option.bind's, then it works.
+  -- i have no idea what causes the bug though.
+  simp only [gothere]
+  try simp (disch := intros; lambda_solve; try trivial) only [Pmatch2Def1]
+  simp only [goback]
+  -- is it recursively doing simp inside the dispatch?
+  --
+  simp only [means, means', means_prog, runProg,
+    runProgDefinitionRet, runProgDefinitionRec, collectOptionDef] at rec1
+  --
+  rewrite [rec1]
+  --
+  simp only [means, means', means_prog, runProg,
+    runProgDefinitionRet, runProgDefinitionRec, collectOptionDef] at rec2
+  normalize
+  rewrite [rec2]
+  simp [Option.bind, collectOptionDef]
+  --
+  --
+
+axiom unknown : Prop
+axiom hole.{u} {T : Type u} : T
+
+-- trying to isolate the nontermination problem
+example
+  (A B : QTerm)
+  : ((collectOption fun i ↦
+          runProgImpl (means_prog fun ty ↦ none)
+            (Pmatch2 (fun (A_1 B : QTerm) ↦ A = <Pi {A_1} {B} >)
+              (fun _ _ ↦ .Ret none)
+              (.Ret none))).bind
+      fun a ↦
+      (collectOption fun i ↦
+            runProgImpl (means_prog fun ty ↦ none)
+              (Pmatch2 (fun (A B_1 : QTerm) ↦ B = <Pi {A} {B_1} >)
+                (fun _ _ ↦ .Ret none)
+                (.Ret none))).bind
+        fun a_1 ↦ some fun f ↦ ∀ (a_2 : QTerm) (inA : a PUnit.unit a_2), a_1 a_2 (< {f} {a_2} >)) =
+    (none : Option (QTerm → Prop))
+  := by
+  --
+  -- Tactic `simp` failed with a nested error:
+  -- (deterministic) timeout at `«tactic execution»`, maximum number of heartbeats (200000) has been reached
+  -- simp (disch := intros; lambda_solve; try trivial) only [Pmatch2Def1]
   --
   sorry
+
+-- can i isolate it more?
+example
+  (A B : QTerm)
+  : ((Pmatch2 (fun (A_1 B : QTerm) ↦ A = <Pi {A_1} {B} >)
+              (fun _ _ ↦ none)
+              none).bind
+      fun (a : Nat) ↦
+              (Pmatch2 (fun (A B_1 : QTerm) ↦ B = <Pi {A} {B_1} >)
+                (fun _ _ ↦ none)
+                none).bind
+        fun (a_1 : Nat) ↦ none) =
+    (none : Option Nat)
+  := by
+  --
+  -- Tactic `simp` failed with a nested error:
+  -- (deterministic) timeout at `«tactic execution»`, maximum number of heartbeats (200000) has been reached
+  -- simp (disch := intros; lambda_solve; try trivial) only [Pmatch2Def1]
+  --
+  sorry
+
+-- gives a different error but still very slow
+example
+  (A B : QTerm)
+  : ((Pmatch2 (fun (A_1 B : QTerm) ↦ unknown)
+              (fun _ _ ↦ none)
+              none).bind
+      fun (_ : Nat) ↦
+              (Pmatch2 (fun (A B_1 : QTerm) ↦ B = <Pi {A} {B_1} >)
+                (fun _ _ ↦ none)
+                none)) =
+    (none : Option Nat)
+  := by
+  --
+  -- just says `simp` made no progress
+  -- but takes a while, so still represents a bug i think?
+  -- simp (disch := intros; lambda_solve; try trivial) only [Pmatch2Def1]
+  --
+  sorry
+
+axiom mybind.{u_1, u_2} {α : Type u_1} {β : Type u_2} : Option α → (α → Option β) → Option β
+
+namespace TestError
+@[inline] protected def mybind2 : Option α → (α → Option β) → Option β
+  | none,   _ => none
+  | some a, f => f a
+end TestError
+
+-- in the below, if i replace Option.bind with mybind or mybind2, then
+-- the simp fails instantly instead of being very slow
+example
+  (A B : QTerm)
+  : (Option.bind (Pmatch2 (fun (A_1 B : QTerm) ↦ unknown)
+              (fun _ _ ↦ none)
+              none)
+      fun (_ : Nat) ↦
+              (Pmatch2 (fun (A B_1 : QTerm) ↦ B = <Pi {A} {B_1} >)
+                (fun _ _ ↦ none)
+                none)) =
+    (none : Option Nat)
+  := by
+  --
+  -- just says `simp` made no progress
+  -- but takes a while, so still represents a bug i think?
+  -- simp (disch := intros; lambda_solve; try trivial) only [Pmatch2Def1]
+  --
+  sorry
+
+-- in this version too,
+-- replacing Option.bind with mybind or TestError.mybind2 makes it fail immediately
+example
+  (A B : QTerm)
+  : (Option.bind (Pmatch2 (fun (A_1 B : QTerm) ↦ A = <Pi {A_1} {B} >)
+              (fun _ _ ↦ none)
+              none)
+      fun (a : Nat) ↦
+              Option.bind (Pmatch2 (fun (A B_1 : QTerm) ↦ B = <Pi {A} {B_1} >)
+                (fun _ _ ↦ none)
+                none)
+        fun (a_1 : Nat) ↦ none) =
+    (none : Option Nat)
+  := by
+  --
+  -- Tactic `simp` failed with a nested error:
+  -- (deterministic) timeout at `«tactic execution»`, maximum number of heartbeats (200000) has been reached
+  -- simp (disch := intros; lambda_solve; try trivial) only [Pmatch2Def1]
+  --
+  sorry
+
+-- so i have no idea what is causing it, but it seems like if i replace
+-- Option.bind with my own version of it then it will fix the problem.
+
+-- let's see if i can shrink it more
+
+example
+  (A B : QTerm)
+  : (Option.bind (Pmatch2 (fun (A_1 B : QTerm) ↦ A = <Pi {A_1} {B} >)
+              (fun _ _ ↦ none)
+              none)
+      fun (a : Nat) ↦
+              (Pmatch2 (fun (A B_1 : QTerm) ↦ B = <Pi {A} {B_1} >)
+                (fun _ _ ↦ none)
+                none)) =
+    (none : Option Nat)
+  := by
+  -- the `simp` made no progress error, but takes a long time to fail.
+  simp (disch := intros; lambda_solve; try trivial) only [Pmatch2Def1]
+  --
+  sorry
+
+/-
+as far as i can figure out, to trigger the bug, you need
+- Option.bind (the one from the standard library, my version doesn't trigger it)
+- one of the Pmatch rewrites
+- lambda_solve in disch.
+-/
